almost finish coroutine example

theories/coroutine_example.v
@@ -11,8 +11,10 @@ Require Import refframe.asm.
 Require Import refframe.itree.
 Require Import refframe.imp_to_asm.
 Require Import refframe.coroutine.
+Require Import refframe.print.
 Require Import refframe.compiler.compiler.
 
+Local Open Scope Z_scope.
 (***
 void stream_inner(int n) {
   gtyield_with_val(n);
@@ -34,28 +36,32 @@ int main(void)
 }
 ***)
 
-Definition stream_addr: Z := 400.
-Definition main_addr: Z := 500.
-Definition print_addr: Z := 600.
+Definition stream_addr: Z := 700.
+Definition main_addr: Z := 800.
 
 Definition stream_imp: fndef := {|
   fd_args := [("n")];
   fd_vars := [];
   fd_body := LetE "_" (imp.Call "yield" [Var "n"]) $
-             (imp.Call "stream" [(BinOp (Var "n") AddOp (Val $ ValNum 1))]);
+             LetE "n'" (BinOp (Var "n") AddOp (Val $ ValNum 1)) $
+             (imp.Call "stream" [Var "n'"]);
   fd_static := I
 |}.
+Definition stream_prog : gmap string fndef :=
+  <["stream" := stream_imp]> $ ∅.
 
 Definition main_imp: fndef := {|
   fd_args := [];
   fd_vars := [];
-  fd_body := LetE "x" (imp.Call "yield" [Val $ ValNum 0]) $
+  fd_body := LetE "x" (imp.Call "yield" [Val $ ValNum 1]) $
              LetE "_" (imp.Call "print" [(Var "x")]) $
              LetE "y" (imp.Call "yield" [Val $ ValNum 0]) $
              LetE "_" (imp.Call "print" [(Var "y")]) $
-             (Val $ ValNum (-1));
+             (Val $ ValNum 0);
   fd_static := I
 |}.
+Definition main_prog : gmap string fndef :=
+  <["main" := main_imp]> $ ∅.
 
 Definition all_f2i : gmap string Z :=
   <["yield"  := yield_addr]> $
@@ -70,26 +76,250 @@ Definition stream_asm : gmap Z asm_instr :=
 Definition main_asm : gmap Z asm_instr :=
   deep_to_asm_instrs main_addr ltac:(i2a_compile all_f2i main_imp).
 
+Definition stream_asm_dom : gset Z := locked (dom _) stream_asm.
+Definition main_asm_dom : gset Z := locked (dom _) main_asm.
+
 Lemma stream_asm_refines_imp :
   trefines (MS asm_module (initial_asm_state stream_asm))
            (MS (imp_to_asm (dom _ stream_asm) {["stream"]} all_f2i imp_module)
                (initial_imp_to_asm_state ∅ imp_module (initial_imp_state (<["stream" := stream_imp]> ∅)))).
-Proof.
-  apply: compile_correct; [|done|..].
-  - by vm_compute.
-  - by vm_compute.
-  - move => ??. rewrite /all_f2i !lookup_insert_Some !lookup_empty.
-    move => ?. destruct_all?; simplify_eq; compute_done.
-Qed.
+Proof. apply: compile_correct; [|done|..]; compute_done. Qed.
 
 Lemma main_asm_refines_imp :
   trefines (MS asm_module (initial_asm_state main_asm))
            (MS (imp_to_asm (dom _ main_asm) {["main"]} all_f2i imp_module)
                (initial_imp_to_asm_state ∅ imp_module (initial_imp_state (<["main" := main_imp]> ∅)))).
+Proof. apply: compile_correct; [|done|..]; compute_done. Qed.
+
+Definition main_itree : itree (moduleE imp_event unit) unit :=
+  '(f, vs, h) ← TReceive (λ '(f, vs, h), (Incoming, EICall f vs h));;;
+  TAssume (f = "main");;;;
+  TAssume (vs = []);;;;
+  TVis (Outgoing, EICall "print" [ValNum 1] h);;;;
+  e ← TExist _;;;
+  TVis (Incoming, e);;;;
+  TAssume (if e is EIReturn _ _ then true else false);;;;
+  TVis (Outgoing, EICall "print" [ValNum 2] (heap_of_event e));;;;
+  e ← TExist _;;;
+  TVis (Incoming, e);;;;
+  TAssume (if e is EIReturn _ _ then true else false);;;;
+  TVis (Outgoing, EIReturn (ValNum 0) (heap_of_event e));;;;
+  TUb.
+Local Ltac go :=
+  clear_itree.
+Local Ltac go_s :=
+  tstep_s; go.
+Local Ltac go_i :=
+  tstep_i; go.
+
+Lemma main_refines_itree :
+  trefines (MS (coro_prod {["main"]} {["stream"]} imp_module imp_module)
+              (initial_coro_prod_state "stream" imp_module imp_module
+              (initial_imp_state main_prog) (initial_imp_state stream_prog)))
+           (MS (mod_itree _ _) (main_itree, tt)).
 Proof.
-  apply: compile_correct; [|done|..].
-  - by vm_compute.
-  - by vm_compute.
-  - move => ??. rewrite /all_f2i !lookup_insert_Some !lookup_empty.
-    move => ?. destruct_all?; simplify_eq; compute_done.
+  apply: tsim_implies_trefines => n0 /=. unfold main_prog, stream_prog.
+  tstep_i => *. destruct_all?; simplify_eq/=.
+  go_s. eexists (_, _, _). go.
+  go_s. split!. go.
+  go_s => ?. go.
+  go_s => ?. go. simplify_eq. rewrite bool_decide_true; [|compute_done].
+  tstep_i. split! => *. simplify_map_eq.
+  tstep_i. split! => *. simplify_map_eq. split!.
+  tstep_i => *. destruct_all?; simplify_eq/=. split; [by econs|].
+  tstep_i. split! => *. destruct_all?; simplify_eq/=.
+  tstep_i. split! => *. simplify_map_eq.
+  tstep_i. split! => *. simplify_map_eq. split!.
+  tstep_i => *. destruct_all?; simplify_eq/=. split; [by econs|].
+  tstep_i. split! => *. destruct_all?; simplify_eq/=.
+  tstep_i. split! => *. destruct_all?; simplify_eq/=.
+  tstep_i.
+  tstep_i. split! => *. destruct_all?; simplify_eq/=.
+  rewrite bool_decide_true; [|compute_done].
+  rewrite bool_decide_false; [|compute_done].
+  go_s. split!. go.
+  tstep_i => e *. destruct_all?; simplify_eq.
+  go_s. eexists _. go.
+  go_s. split!. go.
+  go_s => ?. destruct e => //. go.
+  tstep_i. split! => *. simplify_eq.
+  tstep_i.
+  tstep_i. split! => *. destruct_all?; simplify_eq.
+  tstep_i. split! => *. destruct_all?; simplify_eq.
+  tstep_i.
+  tstep_i.
+  tstep_i.
+  tstep_i. split! => *. simplify_map_eq. split!.
+  tstep_i => *. destruct_all?; simplify_eq/=. split; [by econs|].
+  tstep_i. split! => *. destruct_all?; simplify_eq/=.
+  tstep_i. split! => *. destruct_all?; simplify_eq/=.
+  tstep_i.
+  tstep_i. split! => *. destruct_all?; simplify_eq/=.
+  rewrite bool_decide_true; [|compute_done].
+  rewrite bool_decide_false; [|compute_done].
+  go_s. split!. go.
+  tstep_i => e *. destruct_all?; simplify_eq.
+  go_s. eexists _. go.
+  go_s. split!. go.
+  go_s => ?. destruct e => //. go.
+  tstep_i. split! => *. simplify_eq.
+  tstep_i.
+  tstep_i. split! => *. destruct_all?; simplify_eq.
+  tstep_i. split! => *. destruct_all?; simplify_eq.
+  go_s. split!. go.
+  go_s. done.
+Qed.
+
+Definition stream_sp : Z := 10000.
+Definition stream_gp : Z := 5000.
+Definition stream_regs_init : gmap string Z :=
+  <["SP" := stream_sp]> $
+  <["PC" := stream_addr]> $
+  ∅.
+
+Definition top_level_itree : itree (moduleE asm_event unit) unit :=
+  '(rs, mem) ← TReceive (λ '(rs, mem), (Incoming, EAJump rs mem));;;
+  TAssume (rs !!! "PC" = main_addr);;;;
+  TAssume (rs !!! "R30" ∉ yield_asm_dom ∪ main_asm_dom ∪ stream_asm_dom);;;;
+  TAssume (∃ gp, gp + GUARD_PAGE_SIZE ≤ rs !!! "SP" ∧
+     (i2a_mem_stack_mem (rs !!! "SP") gp ##ₘ
+       (i2a_mem_stack_mem (stream_regs_init !!! "SP") stream_gp ∪ coro_regs_mem stream_regs_init)) ∧
+    i2a_mem_stack_mem (rs !!! "SP") gp ∪
+    (i2a_mem_stack_mem (stream_regs_init !!! "SP") stream_gp ∪ coro_regs_mem stream_regs_init) ⊆ mem);;;;
+  args ← TExist _;;;
+  TAssert (print_args 1 args);;;;
+  TVis (Outgoing, EASyscallCall args);;;;
+  ret ← TReceive (λ ret, (Incoming, EASyscallRet ret));;;
+  args ← TExist _;;;
+  TAssert (print_args 2 args);;;;
+  TVis (Outgoing, EASyscallCall args);;;;
+  ret ← TReceive (λ ret, (Incoming, EASyscallRet ret));;;
+  rs' ← TExist _;;;
+  mem' ← TExist _;;;
+  TVis (Outgoing, EAJump rs' mem');;;;
+  TAssert (rs' !!! "PC" = rs !!! "R30");;;;
+  TAssert (rs' !!! "R0" = 0);;;;
+  TUb.
+
+Lemma top_level_refines_itree :
+  trefines (MS (asm_prod (yield_asm_dom ∪ main_asm_dom ∪ stream_asm_dom)
+                         (dom _ print_asm)
+                         (imp_to_asm (yield_asm_dom ∪ main_asm_dom ∪ stream_asm_dom)
+                                     {["yield"; "main"; "stream"]}
+                                     all_f2i
+                                     (mod_itree _ _)) (mod_itree _ _))
+              (initial_asm_prod_state (imp_to_asm _ _ _ _) (mod_itree _ _)
+                 (initial_imp_to_asm_state
+                    (i2a_mem_stack_mem (stream_regs_init !!! "SP") stream_gp ∪ coro_regs_mem stream_regs_init)
+                    (mod_itree _ _) (main_itree, tt)) (print_itree, tt)))
+           (MS (mod_itree _ _) (top_level_itree, tt)).
+Proof.
+  apply: tsim_implies_trefines => n0 /=.
+  tstep_i => *. case_match; destruct_all?; simplify_eq/=.
+  go_s. eexists (_, _). go.
+  go_s. split!. go.
+  go_s => ?. go. simplify_map_eq'.
+  go_s => ?. go.
+  go_s => -[?[?[??]]]. go.
+  rewrite bool_decide_true. 2: unfold yield_asm_dom, yield_asm, main_asm_dom, stream_asm_dom; unlock; by vm_compute.
+  tstep_i => ??. simplify_eq.
+  tstep_i. eexists true. split; [done|] => /=. eexists initial_heap_state, _, [], [], _, "main". split!.
+  { simplify_map_eq'. done. } 2: done. done.
+  { apply: satisfiable_mono; [by eapply i2a_res_init|].
+    iIntros!. iDestruct select (i2a_mem_auth _) as "$". iFrame.
+    iDestruct (big_sepM_subseteq with "[$]") as "?"; [done|].
+    rewrite big_sepM_union; [|done]. iDestruct!. iFrame.
+    iSplitL; [|iAccu]. by iApply i2a_mem_stack_init. }
+
+  go_i => -[[??]?]. go.
+  go_i => ?. go. simplify_eq.
+  go_i. split!. go.
+  go_i. split!. go.
+  go_i.
+  go_i => *. destruct_all?; simplify_eq.
+  iSatStart. iIntros!.
+  iDestruct (i2a_args_intro with "[$]") as "?"; [done|]. rewrite i2a_args_cons ?i2a_args_nil; [|done].
+  iDestruct!. iSatStop.
+
+  rename select (all_f2i !! _ = Some _) into Hf2i. unfold all_f2i in Hf2i. simplify_map_eq'.
+  rewrite bool_decide_false. 2: unfold yield_asm_dom, yield_asm, main_asm_dom, stream_asm_dom; unlock; by vm_compute.
+  rewrite bool_decide_true. 2: compute_done.
+  go_i.
+  go_i => -[??]. go.
+  go_i => ?. go. simplify_eq.
+  go_i. split!. go.
+  go_i. split. admit. go.
+  go_i => ?. go.
+  go_i => ?. go.
+  go_i => *. go. destruct_all?; simplify_eq.
+
+  go_s. eexists _. go. simplify_map_eq'.
+  go_s. split; [done|]. go.
+  go_s. split; [done|]. go.
+
+  go_i => *. unfold i2a_regs_call in *. case_match; destruct_all?; simplify_eq.
+  go_s. eexists _. go.
+  go_s. split!. go.
+
+  go_i => ?. go.
+  go_i => ?. go. simplify_eq.
+  go_i => *. go. destruct_all?; simplify_map_eq'. rewrite bool_decide_true; [|done].
+  go_i => ??. simplify_eq.
+  go_i. eexists false. split; [done|]. eexists _, _, [ValNum _]. split!. { by simplify_map_eq'. }
+  { split. { by simplify_map_eq'. }
+    apply map_preserved_insert_r_not_in; [compute_done|].
+    apply map_preserved_insert_r_not_in; [compute_done|].
+    apply map_preserved_insert_r_not_in; [compute_done|].
+    done. }
+  { iSatMono. simplify_map_eq'. iFrame. iSplit; [done|]. iAccu. }
+  iSatClear.
+
+  (* TOOD: finish this proof *)
+Admitted.
+
+Lemma complete_refinement :
+  trefines (MS asm_module (initial_asm_state (yield_asm ∪ (main_asm ∪ stream_asm) ∪ print_asm)))
+           (MS (mod_itree _ _) (top_level_itree, tt)).
+Proof.
+  etrans. {
+    apply asm_link_refines_prod. rewrite /yield_asm. unlock. compute_done.
+  }
+  etrans. {
+    apply: asm_prod_trefines; [|done].
+    apply asm_link_refines_prod. rewrite /yield_asm. unlock. compute_done.
+  }
+  etrans. {
+    apply: asm_prod_trefines; [|done].
+    apply: asm_prod_trefines; [done|].
+    apply asm_link_refines_prod. compute_done.
+  }
+  etrans. {
+    apply: asm_prod_trefines.
+    - etrans. {
+        apply: asm_prod_trefines; [done|].
+        apply: asm_prod_trefines.
+        + apply main_asm_refines_imp.
+        + apply stream_asm_refines_imp.
+      }
+      etrans. {
+        rewrite dom_union_L.
+        have ->: dom (gset Z) yield_asm = yield_asm_dom by rewrite /yield_asm_dom; unlock.
+        apply: (coro_spec "stream" stream_regs_init stream_gp).
+        all: unfold yield_asm_dom, yield_asm, i2a_mem_stack_mem; unlock.
+        all: compute_done.
+      }
+      etrans. {
+        apply: imp_to_asm_trefines.
+        apply: main_refines_itree.
+      }
+      done.
+    - apply print_asm_refines_itree.
+  }
+  etrans. {
+    etrans; [|apply top_level_refines_itree].
+    rewrite idemp_L assoc_L 2!dom_union_L.
+    rewrite /yield_asm_dom/main_asm_dom/stream_asm_dom. unlock.
+    done.
+  }
+  done.
 Qed.
