theories/compiler/compiler.v
@@ -53,7 +53,7 @@ Lemma compile_correct f2i f fn dins ins a:
   compile f2i fn = CSuccess dins →
   ins = deep_to_asm_instrs a dins →
   f2i !! f = Some a →
-  (∀ f' i', f2i !! f' = Some i' → ins !! i' = None ↔ f' ≠ f) →
+  map_Forall (λ f' i', ins !! i' = None ↔ f' ≠ f) f2i →
   trefines (MS asm_module (initial_asm_state ins))
            (MS (imp_to_asm (dom _ ins) {[f]} f2i imp_module)
                (initial_imp_to_asm_state ∅ imp_module (initial_imp_state (<[f := fn]> ∅)))).
